refactored lifting pass

deps/poulet4/lib/P4cub/Transformations/Lifting/Lifted.v
@@ -1,48 +1,12 @@
 Require Export Poulet4.P4cub.Syntax.Syntax
         Poulet4.P4cub.Syntax.Shift
-        Poulet4.P4cub.Transformations.Lifting.Statementize
-        Coq.Numbers.DecimalString
-        Coq.Strings.Ascii Coq.Strings.String.
-Import AllCubNotations StringSyntax Field.FieldTactics.
+        Poulet4.P4cub.Transformations.Lifting.Statementize.
+Import AllCubNotations.
 
 Ltac pair_destr :=
   match goal with
   | h: (_,_) = (_,_) |- _ => inv h
   end.
-
-(*
-Ltac translateParserExpr_destr :=
-  match goal with 
-  | |- context [TranslateParserExpr ?e ?env]
-    => destruct (TranslateParserExpr e env) as [? ?] eqn:?; simpl in *
-  end.
-
-Ltac translateCases'_destr :=
-  match goal with 
-  | |- context [TranslateCases' ?c ?env ?i]
-    => destruct (TranslateCases' c env i) as [[? ?] ?] eqn:?; simpl in *
-  end.
- *)
-(*
-Ltac translateStmt_destr :=
-  match goal with
-  | |- context [TranslateStatement ?s ?env]
-    => destruct (TranslateStatement s env) as [? ?] eqn:?; simpl in *
-  end.
- *)
-(*
-Ltac translateArrowE_destr :=
-  match goal with
-  | |- context [TranslateArrowE ?args ?env ?i]
-    => destruct (TranslateArrowE args env i) as [[? ?] ?] eqn:?; simpl in *
-  end.
-
-Ltac translateArgs_destr :=
-  match goal with
-  | |- context [TranslateArgs ?args ?env ?i]
-    => destruct (TranslateArgs args env i) as [[? ?] ?] eqn:?; simpl in *
-  end.
-*)
 
 Ltac lift_e_destr :=
   match goal with
@@ -50,25 +14,6 @@ Ltac lift_e_destr :=
     => destruct (lift_e up e) as [? ?] eqn:?; simpl in *
   end.
 
-(*
-Ltac translateControlDecl_destr := 
-  match goal with
-  | |- context [TranslateControlDecl ?cd ?env]
-    => destruct (TranslateControlDecl cd env) as [[? ?] ?] eqn:?; simpl in *
-  end.
-
-Ltac translateTable_destr := 
-  match goal with
-  | |- context [TranslateTable ?body ?env ?i]
-    => destruct (TranslateTable body env i) as [[? ?] ?] eqn:?; simpl in *
-  end.
-
-Ltac translateTopDecl_destr := 
-  match goal with
-  | |- context [TranslateTopDecl ?td ?env]
-    => destruct (TranslateTopDecl td env) as [? ?] eqn:?; simpl in *
-  end.
-*)
 Ltac lift_e_destr_hyp :=
   match goal with
   | H: context [lift_e ?up ?e] |- _
@@ -94,8 +39,8 @@ Inductive lifted_expr : Expr.e -> Prop :=
 | lifted_error err :
   lifted_expr (Expr.Error err).
 
-Definition lifted_args (args : Expr.args) : Prop :=
-  Forall (pred_paramarg_same lifted_expr) args.
+Definition lifted_arg : paramarg Expr.e Expr.e -> Prop :=
+  pred_paramarg_same lifted_expr.
 
 Variant lifted_lexpr : Expr.e -> Prop :=
   | lifted_lifted_expr e :
@@ -165,7 +110,7 @@ Inductive lifted_stmt : Stmt.s -> Prop :=
   lifted_stmt (Stmt.Seq s1 s2)
 | lifted_call fk args :
   lifted_fun_kind fk ->
-  lifted_args args ->
+  Forall lifted_arg args ->
   lifted_stmt (Stmt.Call fk args)
 | lifted_return eo :
   match eo with
@@ -181,7 +126,7 @@ Inductive lifted_stmt : Stmt.s -> Prop :=
 | lifted_invoke t :
   lifted_stmt (Stmt.Invoke t)
 | lifted_apply x ext_args args :
-  lifted_args args ->
+  Forall lifted_arg args ->
   lifted_stmt (Stmt.Apply x ext_args args).
 
 Variant lifted_control_Decl : Control.d -> Prop :=
@@ -241,7 +186,7 @@ Proof.
   - apply IHe in Heqp as [? ?]; auto.
   - apply IHe in Heqp as [? ?]; auto.
   - apply IHe in Heqp as [? ?]; auto.
-  - destruct (lift_e (List.length l0 + up) e2) as [l2  e2'] eqn:eql2.
+  - destruct (lift_e (length l0 + up) e2) as [l2  e2'] eqn:eql2.
     apply IHe1 in Heqp as [? ?].
     apply IHe2 in eql2 as [? ?].
     pair_destr.
@@ -282,469 +227,171 @@ Proof.
   - apply IHe in Heqp as [? ?]; auto.
 Qed.
 
+Local Hint Resolve lift_e_lifted_expr : core.
+
+Lemma lift_e_list_lifted_expr : forall es es' le up,
+    lift_e_list up es = (le, es') ->
+    Forall lifted_lexpr le /\ Forall lifted_expr es'.
+Proof.
+  intro es; induction es as [| e es ih];
+    intros es' le up h; unravel in *;
+    try lift_e_destr_hyp; try pair_destr; eauto.
+  destruct (lift_e_list (length l + up) es)
+    as [les es''] eqn:eqles; inv h.
+  rewrite Forall_app.
+  apply ih in eqles as [? ?].
+  apply lift_e_lifted_expr in Heqp as [? ?]; auto.
+Qed.
+
+Local Hint Resolve lift_e_list_lifted_expr : core.
+
+Lemma lift_arg_lifted_arg : forall arg arg' le up,
+    lift_arg up arg = (le, arg') ->
+    Forall lifted_lexpr le /\ lifted_arg arg'.
+Proof.
+  intros arg arg' le up h;
+    destruct arg as [e | e | e]; unravel in *;
+    lift_e_destr_hyp; pair_destr;
+    eapply lift_e_lifted_expr; eauto.
+Qed.
+  
+Local Hint Resolve lift_arg_lifted_arg : core.
+
+Lemma rename_arg_lifted_arg : forall ρ arg,
+    lifted_arg arg -> lifted_arg (rename_arg ρ arg).
+Proof.
+  intros ρ [e | e | e] h; unravel in *; auto.
+Qed.
+
+Local Hint Resolve rename_arg_lifted_arg : core.
+
+Lemma lift_args_lifted_args : forall args args' le up,
+    lift_args up args = (le, args') ->
+    Forall lifted_lexpr le /\ Forall lifted_arg args'.
+Proof.
+  intro args; induction args as [| arg args ih];
+    intros args' le up h; unravel in *.
+  - pair_destr; auto.
+  - destruct (lift_arg up arg) as [larg arg'] eqn:eqlarg.
+    destruct (lift_args (length larg + up) args) as [largs args''] eqn:eqlargs.
+    pair_destr. rewrite Forall_app.
+    apply lift_arg_lifted_arg in eqlarg as [? ?].
+    apply ih in eqlargs as [? ?]; auto.
+Qed.
+
+Local Hint Resolve lift_args_lifted_args : core.
+Local Hint Constructors lifted_parser_expr : core.
+
+Lemma lift_trans_lifted_parser_expr : forall e e' le up,
+    lift_trans up e = (le, e') ->
+    Forall lifted_lexpr le /\ lifted_parser_expr e'.
+Proof.
+  intros e e' le up h; destruct e;
+    unravel in *; try lift_e_destr_hyp;
+    pair_destr; auto.
+  apply lift_e_lifted_expr in Heqp as [? ?]; auto.
+Qed.
+
+Local Hint Constructors lifted_fun_kind : core.
+Local Hint Constructors predop : core.
+
+Lemma lift_fun_kind_lifted_fun_kind : forall fk fk' up le,
+    lift_fun_kind up fk = (le, fk') ->
+    Forall lifted_lexpr le /\ lifted_fun_kind fk'.
+Proof.
+  intros fk fk' up le h; destruct fk; unravel in *.
+  - destruct returns as [e |]; try lift_e_destr_hyp; pair_destr; auto.
+    apply lift_e_lifted_expr in Heqp as [? ?]; auto.
+  - destruct (lift_e_list up control_plane_args) as [les es'] eqn:eqles.
+    pair_destr; apply lift_e_list_lifted_expr in eqles as [? ?]; auto.
+  - destruct returns as [e |]; try lift_e_destr_hyp; pair_destr; auto.
+    apply lift_e_lifted_expr in Heqp as [? ?]; auto.
+Qed.
+
+Lemma rename_fun_kind_lifted_fun_kind : forall ρ fk,
+    lifted_fun_kind fk ->
+    lifted_fun_kind (rename_fun_kind ρ fk).
+Proof.
+  intros ρ fk h; inv h; unravel.
+  - constructor; destruct oe; unravel; inv H; auto.
+  - constructor.
+    rewrite sublist.Forall_map; unravel.
+    rewrite Forall_forall in *; eauto.
+  - constructor; destruct oe; unravel; inv H; auto.
+Qed.
+
+Local Hint Resolve rename_fun_kind_lifted_fun_kind : core.
+
 Local Hint Constructors lifted_stmt : core.
 
-  Ltac seq_lift :=
-    match goal with
-    | |- lifted_stmt (_; _ @ _ }-
-      => apply lifted_seq
-    end.
+Lemma unwind_vars_lifted : forall le s,
+    Forall lifted_lexpr le ->
+    lifted_stmt s ->
+    lifted_stmt (unwind_vars le s).
+Proof.
+  intro le; induction le as [| e le ih];
+    intros s hle hs; inv hle; unravel; auto.
+Qed.
 
-  Local Hint Resolve TransformExpr_lifted_expr : core.
+Local Hint Resolve unwind_vars_lifted : core.
 
-  Lemma TransformExprList'_TransformExpr_lifted_expr : forall es env i,
-      Forall
-        lifted_expr
-        (snd
-           (fst
-              (TransformExprList'
-                 TransformExpr es env i))).
-  Proof.
-    auto.
-  Qed.
+Lemma lift_s_lifted_stmt : forall s up, lifted_stmt (lift_s up s).
+Proof.
+  intro s; induction s; intro up; unravel; auto.
+  - destruct e as [e |]; auto.
+    lift_e_destr; apply lift_e_lifted_expr in Heqp.
+    intuition.
+  - destruct (lift_trans up e) as [le e'] eqn:eqle.
+    apply lift_trans_lifted_parser_expr in eqle as [? ?].
+    intuition.
+  - do 2 lift_e_destr.
+    apply lift_e_lifted_expr in Heqp as [? ?], Heqp0 as [? ?].
+    apply unwind_vars_lifted; auto.
+    rewrite Forall_app; auto.
+  - destruct (lift_fun_kind up call) as [lfk fk'] eqn:eqfk.
+    destruct (lift_args (length lfk + up) args) as [largs args'] eqn:eqargs.
+    apply lift_fun_kind_lifted_fun_kind in eqfk as [? ?].
+    apply lift_args_lifted_args in eqargs as [? ?].
+    apply unwind_vars_lifted; auto.
+    rewrite Forall_app; auto.
+  - destruct (lift_args up args) as [largs args'] eqn:eqargs.
+    apply lift_args_lifted_args in eqargs as [? ?]; auto.
+  - destruct expr as [t | e]; auto.
+    lift_e_destr. apply lift_e_lifted_expr in Heqp as [? ?]; auto.
+  - lift_e_destr. apply lift_e_lifted_expr in Heqp as [? ?]; auto.
+Qed.
 
-  Local Hint Resolve TransformExprList'_TransformExpr_lifted_expr : core.
-  
-  Lemma TransformFields'_TransformExpr_lifted_expr : forall es env i,
-      F.predfs_data
-        lifted_expr
-        (snd (fst (TransformFields' TransformExpr es env i))).
-  Proof.
-    auto.
-  Qed.
+Local Hint Resolve lift_s_lifted_stmt : core.
 
-  Local Hint Resolve TransformFields'_TransformExpr_lifted_expr : core.
+Ltac hyp_f_equal Heqp func:= 
+  apply f_equal with (f := fst) in Heqp; apply f_equal with (f := func) in Heqp; simpl in Heqp;
+  rewrite <- Heqp; auto.
 
-  Lemma TransformExprList'_lifted_stmt_Forall :
-    forall es,
-      Forall
-        (fun e => forall env,
-             lifted_stmt (fst (fst (lift_e up e)))) es ->
-      forall env i,
-        lifted_stmt (fst (fst (TransformExprList' TransformExpr es env i))).
-  Proof.
-    unfold TransformExprList';
-      intros es H; ind_list_Forall;
-        intros env i; simpl in *; auto.
-    intuition; fold_destr.
-    specialize H with env i.
-    rewrite Hfoldl in H; simpl in *; clear Hfoldl.
-    specialize H2 with t. transformExpr_destr.
-    auto.
-  Qed.
+Ltac hyp_f_equal_fst Heqp:= 
+  apply f_equal with (f := fst) in Heqp; apply f_equal with (f := fst) in Heqp; simpl in Heqp;
+  rewrite <- Heqp; auto.
 
-  Local Hint Resolve TransformExprList'_lifted_stmt_Forall : core.
+Ltac hyp_f_equal_snd Heqp:= 
+  apply f_equal with (f := fst) in Heqp; apply f_equal with (f := snd) in Heqp; simpl in Heqp;
+  rewrite <- Heqp; auto.
 
-  Lemma TransformFields'_lifted_stmt_Forall :
-    forall fields,
-      F.predfs_data
-        (fun e => forall env,
-             lifted_stmt (fst (fst (lift_e up e)))) fields ->
-      forall env i,
-        lifted_stmt (fst (fst (TransformFields' TransformExpr fields env i))).
-  Proof.
-    unfold TransformFields', Field.fold;
-      intros es H; ind_list_predfs;
-        intros env i; simpl in *; auto.
-    intuition. fold_destr.
-    specialize H with env i.
-    rewrite Hfoldl in H; simpl in *; clear Hfoldl.
-    specialize H2 with t. transformExpr_destr.
-    auto.
-  Qed.
+Local Hint Constructors lifted_control_Decl : core.
 
-  Local Hint Resolve TransformFields'_lifted_stmt_Forall : core.
-  
-  Lemma TransformExpr_lifted_stmt : forall e env,
-      lifted_stmt (fst (fst (lift_e up e))).
-  Proof.
-    intro e; induction e using custom_e_ind;
-      intro env; unravel in *;
-        repeat transformExpr_destr;
-        repeat seq_lift; auto;
-          try (specialize IHe with env;
-               transformExpr_destr_hyp_rewrite;
-               assumption);
-          try (specialize IHe with env;
-               transformExpr_destr_hyp_rewrite;
-               apply f_equal with (f:= (snd ∘ fst)) in Heqp;
-               unravel in *; rewrite <- Heqp; auto; assumption).
-    - specialize IHe1 with env;
-        transformExpr_destr_hyp_rewrite; assumption.
-    - specialize IHe2 with t;
-        transformExpr_destr_hyp_rewrite; assumption.
-    - specialize IHe1 with env;
-        specialize IHe2 with t;
-        transformExpr_destr_hyp_rewrite;
-        apply f_equal with (f:= snd ∘ fst) in Heqp;
-        apply f_equal with (f:= snd ∘ fst) in Heqp0.
-      unravel in *; rewrite <- Heqp, <- Heqp0; auto.
-    - apply f_equal with (f := fst ∘ fst) in Heqp; unravel in *.
-      rewrite <- Heqp; auto.
-    - apply lifted_tuple.
-      apply f_equal with (f := snd ∘ fst) in Heqp; unravel in *.
-      rewrite <- Heqp; auto.
-    - apply f_equal with (f := fst ∘ fst) in Heqp; unravel in *.
-      rewrite <- Heqp; auto.
-    - apply lifted_struct.
-      apply f_equal with (f := snd ∘ fst) in Heqp; unravel in *.
-      rewrite <- Heqp; auto.
-    - apply f_equal with (f := fst ∘ fst) in Heqp; unravel in *.
-      rewrite <- Heqp; auto.
-    - apply f_equal with (f := fst ∘ fst) in Heqp0; unravel in *.
-      rewrite <- Heqp0; auto.
-    - apply lifted_header.
-      + apply f_equal with (f := snd ∘ fst) in Heqp0; unravel in *.
-        rewrite <- Heqp0; auto.
-      + apply f_equal with (f := snd ∘ fst) in Heqp; unravel in *.
-        rewrite <- Heqp; auto.
-    - apply f_equal with (f := fst ∘ fst) in Heqp; unravel in *.
-      rewrite <- Heqp; auto.
-    - apply lifted_stack.
-      apply f_equal with (f:=snd ∘ fst) in Heqp; unravel in *.
-      rewrite <- Heqp; auto.
-  Qed.
+Lemma lift_control_decl_lifted_control_Decl : forall cd,
+    lifted_control_Decl (lift_control_decl cd).
+Proof.
+  intros cd; destruct cd; unravel; auto.
+  constructor. (* TODO: table keys are sad *)
+Abort.
 
-  Local Hint Resolve TransformExpr_lifted_stmt : core.
+Local Hint Constructors lifted_top_Decl : core.
 
-  Ltac hyp_f_equal Heqp func:= 
-    apply f_equal with (f := fst) in Heqp; apply f_equal with (f := func) in Heqp; simpl in Heqp;
-      rewrite <- Heqp; auto.
-  
-  Ltac hyp_f_equal_fst Heqp:= 
-    apply f_equal with (f := fst) in Heqp; apply f_equal with (f := fst) in Heqp; simpl in Heqp;
-      rewrite <- Heqp; auto.
-  
-  Ltac hyp_f_equal_snd Heqp:= 
-    apply f_equal with (f := fst) in Heqp; apply f_equal with (f := snd) in Heqp; simpl in Heqp;
-      rewrite <- Heqp; auto.
-
-  Lemma TranslateArgs_lifted_stmt : forall (a : Expr.args ) env i,
-  lifted_stmt (fst (fst (TranslateArgs a env i))).
-  Proof.
-    intros a i. induction a;
-      intro env; simpl.
-      - constructor.
-      - destruct a. destruct (TranslateArgs a0 i env) eqn:Hs2. destruct p0. transformExpr_destr. 
-        constructor.
-        + hyp_f_equal_fst Hs2.
-        + hyp_f_equal_fst Heqp0.
-  Qed.
-
-  Local Hint Resolve TranslateArgs_lifted_stmt : core.
-
-  Lemma TranslateArrowE_lifted_stmt : forall (args : Expr.arrowE ) env i, 
-  lifted_stmt (fst (fst (TranslateArrowE args env i))).
-  Proof.
-    intros [pas returns] i env; simpl.
-    destruct (TranslateArgs pas i env) eqn:Hs1. destruct p. destruct returns.
-    - transformExpr_destr. constructor.
-      + hyp_f_equal_fst Hs1.
-      + hyp_f_equal_fst Heqp.
-    - simpl. hyp_f_equal_fst Hs1. 
-  Qed.
-
-  Local Hint Resolve TranslateArrowE_lifted_stmt : core.
-
-  Lemma TranslateArgs_lifted_expr : forall pas env i,
-      Field.predfs_data (pred_paramarg_same lifted_expr) (snd (fst (TranslateArgs pas i env))).
-  Proof.
-    intros pas i. induction pas; intro env; simpl.
-    - constructor.
-    - destruct a. translateArgs_destr. transformExpr_destr.
-      destruct p; unfold F.predfs_data, F.predf_data in *; 
-    unravel in *; rewrite Forall_app; split; try hyp_f_equal_snd Heqp0; repeat constructor;
-    simpl; unfold pred_paramarg_same, pred_paramarg; hyp_f_equal_snd Heqp1.
-  Qed.
-
-  Local Hint Resolve TranslateArgs_lifted_expr : core.
-
-  Local Hint Constructors predop : core.
-
-  Lemma TransformExpr_lifted_args : forall pas i (e:Expr.e ) t env,
-      lifted_args {|paramargs:=snd (fst (TranslateArgs pas i env));
-                    rtrns:=Some (snd (fst (TransformExpr e t)))|}.
-  Proof.
-    unfold lifted_args.
-    intros pas i e t env; simpl; auto.
-  Qed.
-
-  Local Hint Resolve TransformExpr_lifted_args : core.
-   
-  Lemma TranslateArrowE_lifted_args : forall (args : Expr.arrowE ) env i, 
-  lifted_args (snd (fst (TranslateArrowE args env i))).
-  Proof.
-    intros [pas returns] i env; simpl.
-    destruct (TranslateArgs pas i env) eqn:Hs1;
-      destruct p eqn:Hs2; destruct returns eqn:Hs3; cbn.
-    - transformExpr_destr. hyp_f_equal_snd Heqp0. hyp_f_equal_snd Hs1.
-    - hyp_f_equal_snd Hs1. unfold lifted_args; split; cbn; auto.
-  Qed.
-
-  Local Hint Resolve TranslateArrowE_lifted_args : core.
-
-  Lemma TranslateStmt_lifted_stmt : forall (s : Stmt.s ) (env:VarNameGen.t),
-  lifted_stmt (fst (TranslateStatement s env)).
-  Proof.
-  intros s. induction s; intros env; try simpl; auto; repeat transformExpr_destr.
-  - destruct expr.
-    + simpl. auto.
-    + transformExpr_destr. constructor. 
-      * hyp_f_equal_fst Heqp. 
-      * constructor. hyp_f_equal_snd Heqp.
-  - repeat constructor. 
-    + hyp_f_equal_fst Heqp.
-    + hyp_f_equal_fst Heqp0.
-    + hyp_f_equal_snd Heqp.   
-    + hyp_f_equal_snd Heqp0.
-  - repeat translateStmt_destr. constructor.
-    + hyp_f_equal_fst Heqp.
-    + constructor. 
-      * hyp_f_equal_snd Heqp. 
-      * hyp_f_equal Heqp0 (fun x:(Stmt.s ) => x).
-      * hyp_f_equal Heqp1 (fun x:(Stmt.s ) => x). 
-  - repeat translateStmt_destr. constructor. 
-    + hyp_f_equal Heqp (fun x:(Stmt.s ) => x).
-    + hyp_f_equal Heqp0 (fun x:(Stmt.s ) => x). 
-  - translateStmt_destr. constructor. hyp_f_equal Heqp (fun x:(Stmt.s ) => x).
-  - translateArrowE_destr. constructor.
-    + hyp_f_equal_fst Heqp.
-    + constructor. hyp_f_equal_snd Heqp. 
-  - translateArrowE_destr. constructor.
-    + hyp_f_equal_fst Heqp.
-    + hyp_f_equal_snd Heqp.
-  - translateArgs_destr. constructor.
-    + hyp_f_equal_fst Heqp. 
-    + hyp_f_equal_snd Heqp. 
-  - destruct e.
-    + transformExpr_destr. constructor.
-      * hyp_f_equal_fst Heqp.
-      * hyp_f_equal_snd Heqp.
-    + simpl. auto.
-  - translateArgs_destr. constructor.
-    + hyp_f_equal_fst Heqp.
-    + hyp_f_equal_snd Heqp. 
-  - repeat constructor.
-    + hyp_f_equal_fst Heqp.
-    + hyp_f_equal_snd Heqp.
-  Qed.
-
-  Local Hint Resolve TranslateStmt_lifted_stmt : core.
-
-
-  Lemma TranslateCases_lifted_stmt : forall (translateParserE : Parser.e  -> VarNameGen.t -> (Stmt.s ) * Parser.e  * VarNameGen.t)
-  (cases: Field.fs Parser.pat (Parser.e )),
-  F.predfs_data (fun pe => forall env, lifted_stmt (fst (fst (translateParserE pe env)))) cases -> 
-  forall (env: VarNameGen.t) (: ), 
-  lifted_stmt (fst (fst (TranslateCases' translateParserE cases env i))).
-  Proof.
-  intros translateParserE cases Hpte; ind_list_predfs; intros. 
-  - simpl. auto.
-  - simpl. translateCases'_destr. destruct (translateParserE e t) eqn: HS1.
-  destruct p0. simpl. constructor.
-    + hyp_f_equal_fst Heqp0.
-    + hyp_f_equal_fst HS1.
-  Qed.
-
-  Local Hint Resolve TranslateCases_lifted_stmt : core.
-
-  Lemma TranslateParserExpr_lifted_stmt : forall (e : Parser.e ) (env:VarNameGen.t),
-  lifted_stmt (fst (fst (TranslateParserExpr e env))).
-  Proof.
-  intros e. induction e using pe_ind; intro env; try simpl; auto.
-  transformExpr_destr. translateParserExpr_destr. destruct p eqn:Hs0. destruct (TranslateCases' TranslateParserExpr cases t0 i) eqn:Hs1.
-  destruct p0 eqn: Hs2. simpl. repeat constructor; auto. 
-  - hyp_f_equal_fst Heqp.
-  - hyp_f_equal_fst Heqp0.
-  - hyp_f_equal_fst Hs1.
-  Qed. 
-
-  Local Hint Resolve TranslateParserExpr_lifted_stmt : core.
-
-  Lemma TranslateCases_lifted_expr : forall (translateParserE : Parser.e  -> VarNameGen.t -> (Stmt.s ) * Parser.e  * VarNameGen.t)
-  (cases: Field.fs Parser.pat (Parser.e )),
-  F.predfs_data (fun pe => forall env, lifted_parser_expr (snd (fst (translateParserE pe env)))) cases -> 
-  forall (env: VarNameGen.t) (: ), 
-  F.predfs_data lifted_parser_expr (snd (fst (TranslateCases' translateParserE cases env i))).
-  Proof.
-  intros translateParserE cases Hpte; ind_list_predfs; intros; unfold F.predfs_data in *; 
-  unfold F.predf_data in *; unravel in *; auto.
-  translateCases'_destr. destruct (translateParserE e t) eqn: HS1.
-  destruct p0. simpl. rewrite Forall_app. split.
-    + hyp_f_equal_snd Heqp0.
-    + constructor; auto. simpl. hyp_f_equal_snd HS1.
-  Qed.
-
-  Local Hint Resolve TranslateCases_lifted_expr : core.
-
-  Lemma TranslateParserExpr_lifted_parser_expr : forall (e : Parser.e ) (env:VarNameGen.t),
-  lifted_parser_expr (snd (fst (TranslateParserExpr e env))).
-  Proof.
-  intros e. induction e using pe_ind; intro env; try simpl; auto.
-  transformExpr_destr. translateParserExpr_destr. destruct p.
-  translateCases'_destr. constructor.
-  - hyp_f_equal_snd Heqp.
-  - hyp_f_equal_snd Heqp0.
-  - hyp_f_equal_snd Heqp1.   
-  Qed. 
-
-  Local Hint Resolve TranslateParserExpr_lifted_parser_expr : core.
-
-  Lemma TranslateParserState_lifted_stmt :
-    forall (parser_state: Parser.state_block ) (env : VarNameGen.t),
-      lifted_parser_state (fst (TranslateParserState parser_state env)).
-  Proof.
-    intros [s e] env; simpl; translateStmt_destr; translateParserExpr_destr.
-    destruct p. simpl. unfold lifted_parser_state; split; cbn; try constructor.
-    - hyp_f_equal Heqp (fun x:(Stmt.s ) => x).
-    - hyp_f_equal_fst Heqp0.
-    - hyp_f_equal_snd Heqp0.
-  Qed.
-
-  Local Hint Resolve TranslateParserState_lifted_stmt : core.
-
-  Lemma TranslateParserStates_lifted_stmt :
-    forall (parser_states: Field.fs string (Parser.state_block )) (env : VarNameGen.t),
-      lifted_parser_states (fst (TranslateParserStates parser_states env)).
-  Proof.
-    induction parser_states; intros; simpl in *.
-    - constructor.
-    - destruct a.
-      unfold lifted_parser_states, F.predfs_data.
-      destruct (TranslateParserStates parser_states env) as [prev_states env_prev] eqn:?.
-      destruct (TranslateParserState s0 env_prev) as [s' env_state] eqn:?.
-      apply Forall_app; split.
-      + apply (f_equal fst) in Heqp.
-        simpl (fst _) in Heqp.
-        rewrite <- Heqp.
-        apply IHparser_states.
-      + constructor; auto.
-        unfold F.predf_data.
-        change _ with (lifted_parser_state s').
-        apply (f_equal fst) in Heqp0.
-        simpl (fst _) in Heqp0.
-        rewrite <- Heqp0.
-        auto.
-  Qed.
-
-  Local Hint Resolve TranslateParserStates_lifted_stmt : core.
-
-  Lemma TranslateTable_lifted_stmt :
-    forall (t: Control.table ) (env: VarNameGen.t) (: ),
-      lifted_stmt (fst (fst (TranslateTable t env i))).
-  Proof.
-    intros [ky acts] env i; cbn; fold_destr; clear acts.
-    hyp_f_equal_fst Hfoldl.
-    clear Hfoldl l t s.
-    generalize dependent env.
-    induction ky as [| [e mk] ky IHky]; intros env; simpl in *; auto.
-    fold_destr; transformExpr_destr.
-    specialize IHky with env.
-    rewrite Hfoldl in IHky; simpl in *.
-    hyp_f_equal_fst Heqp.
-  Qed.
-
-  Local Hint Resolve TranslateTable_lifted_stmt : core.
-
-  Lemma TranslateTable_lifted_table :
-    forall (t: Control.table ) (env: VarNameGen.t) (: ),
-      lifted_table (snd (fst (TranslateTable t env i))).
-  Proof.
-    intros [ky acts] env i; cbn; fold_destr.
-    hyp_f_equal_snd Hfoldl.
-    clear Hfoldl l t s.
-    generalize dependent env.
-    induction ky as [| [e mk] ky IHky]; intros env; simpl in *.
-    - constructor.
-    - fold_destr; transformExpr_destr.
-      specialize IHky with env.
-      rewrite Hfoldl in IHky; simpl in *.
-      constructor.
-      + hyp_f_equal_snd Heqp.
-      + inversion IHky; simpl in *; subst l; auto.
-  Qed.
-
-  Local Hint Resolve TranslateTable_lifted_table : core.
-
-  Lemma TranslateControlDecl_lifted_stmt : forall (cd : Control.d ) (env : VarNameGen.t),
-      lifted_stmt (fst (fst (TranslateControlDecl cd env))).
-  Proof.
-    intro cd. induction cd; intro env; simpl; auto.  
-    - translateStmt_destr. auto. 
-    - simpl. translateTable_destr. hyp_f_equal_fst Heqp.
-    - repeat translateControlDecl_destr. constructor.
-      + hyp_f_equal_fst Heqp.
-      + hyp_f_equal_fst Heqp0.
-  Qed.  
-
-  Local Hint Resolve TranslateControlDecl_lifted_stmt : core.
-
-  Lemma TranslateControlDecl_lifted_decl : forall (cd : Control.d ) (env : VarNameGen.t),
-      lifted_control_Decl (snd (fst (TranslateControlDecl cd env))).
-  Proof.
-    intro cd. induction cd; intro env; simpl; auto.  
-    - translateStmt_destr. 
-      constructor.
-      replace s with (fst (TranslateStatement body env))
-        by (rewrite Heqp; exact eq_refl).
-      eauto.
-    - translateTable_destr.
-      constructor.
-      hyp_f_equal_snd Heqp.
-    - repeat translateControlDecl_destr. constructor.
-      + hyp_f_equal_snd Heqp.
-      + hyp_f_equal_snd Heqp0.
-  Qed.  
-  
-  Local Hint Resolve TranslateControlDecl_lifted_decl : core.
-
-  Lemma TranslateTopDecl_lifted_top_Decl : forall (td : TopDecl.d ) (env : VarNameGen.t),
-      lifted_top_Decl (fst (TranslateTopDecl td env)).
-  Proof.
-    induction td; intros; simpl; try solve [constructor].
-    - translateControlDecl_destr.
-      translateStmt_destr.
-      constructor.
-      + hyp_f_equal_snd Heqp.
-      + constructor.
-        * hyp_f_equal_fst Heqp.
-        * replace s0 with (fst (TranslateStatement apply_blk t))
-            by (rewrite Heqp0; exact eq_refl).
-          auto.
-    - (* annoying--can't write (... start env) here because start gets
-      grabbed by some notation and then fails to parse *)
-      destruct (TranslateParserState _ env) as [start' env_start] eqn:?.
-      destruct (TranslateParserStates states env_start) as [states' env_states] eqn:?.
-      constructor.
-      + apply (f_equal fst) in Heqp.
-        simpl (fst _) in Heqp.
-        rewrite <- Heqp.
-        auto.
-      + apply (f_equal fst) in Heqp0.
-        simpl (fst _) in Heqp0.
-        rewrite <- Heqp0.
-        eauto.
-    - translateStmt_destr.
-      constructor; auto.
-      replace s with (fst (TranslateStatement body env))
-        by (rewrite Heqp; exact eq_refl).
-      auto.
-    - translateTopDecl_destr.
-      translateTopDecl_destr.
-      replace d with (fst (TranslateTopDecl td1 env))
-        by (rewrite Heqp; exact eq_refl).
-      replace d0 with (fst (TranslateTopDecl td2 t))
-        by (rewrite Heqp0; exact eq_refl).
-      constructor; auto.
-  Qed.
-
-  Local Hint Resolve TranslateTopDecl_lifted_top_Decl : core.
-
-  Lemma TranslateProgram_lifted_top_Decl : forall (prog: TopDecl.d ),
-      lifted_top_Decl (TranslateProgram prog).
-  Proof.
-    unfold TranslateProgram.
-    auto.
-  Qed.
-
-End Lifted.
+Lemma lift_top_decl_lifted_top_Decl : forall td,
+    lifted_top_Decl (lift_top_decl td).
+Proof.
+  intro td; destruct td; unravel in *; auto.
+  - constructor; auto. (* TODO: tables?? *) admit.
+  - constructor; auto.
+    rewrite sublist.Forall_map; unravel.
+    rewrite Forall_forall in *; eauto.
+Abort.
